
Section 1.3 - Regular Expressions

CSC 320

Regular Expressions

The *regular expressions* over an alphabet Σ are exactly all strings over the alphabet $\Sigma \cup \{ (,), \emptyset, \varepsilon, \cup, * \}$ that can be obtained as follows:

1. \emptyset , ε , and the members of Σ are regular expressions.
 2. If R and S are regular expressions, then so is $R \cdot S$ and so is $R \cup S$.
 3. If R is a regular expression, then so is R^* .
 4. If R is a regular expression, then so is (R) .
- $*$ has the highest precedence, followed by \cdot , followed by \cup .

Both \cdot and \cup are associative.

Some Abbreviations and Alternatives

- We sometimes write $+$ for \cup (sometimes $|$ is used as well, but we won't use this.)
- We sometimes write RS for $R \cdot S$
- We write R^+ to denote RR^*

Languages Represented by Regular Expressions

Every regular expression represents a language. We define L to be a function which maps any regular expression to a language, as follows:

- $L(\emptyset) = \emptyset$, $L(\varepsilon) = \{\varepsilon\}$ and $L(a) = \{a\}$ for all $a \in \Sigma$.
- If R and S are regular expressions, then $L(RS) = L(R)L(S)$, and $L(R \cup S) = L(R) \cup L(S)$.
- If R is a regular expression, then $L(R^*) = (L(R))^*$.
- If R is a regular expression, then $L((R)) = L(R)$
- We often don't write the $L(E)$ but just put the E to refer to the language corresponding to E .

Examples of Languages Defined by Regular Expressions

1. 0^*10^*
2. $\Sigma^*001\Sigma^*$
3. $\{w \in \Sigma^* \mid w \text{ ends with a } 1\}$
4. $\{w \in \Sigma^* \mid w \text{ does not contain the substring } 10\}$.

Equivalence of FA's and Regular Expressions

- *Theorem: A language is regular if and only if (\Leftrightarrow) some regular expression describes it.*
- **Proof:** We show each direction separately.
- (\Leftarrow) First, we show that if a language is described by a regular expression R then there is an NFA which recognizes it.

Base Case

- $R = \emptyset$
- $R = \varepsilon$
- $R = a, \quad a \in \Sigma$

Induction

Suppose S, T are regular expressions. We assume for induction that there are NFAs M_S, M_T such that $L(S) = L(M_S)$ and $L(T) = L(M_T)$. For each case below, we need to construct an NFA M_R such that $L(M_R) = L(R)$.

1. $R = S \cup T$

2. $R = S \cdot T$

3. $R = S^*$

4. $R = (S)$

Example – Regular Expression to NFA

Consider the regular expression $(ab \cup aba)^*$.

1. NFA's for ab and aba :

2. NFA for $(ab \cup aba)$

Example – Regular Expression to NFA

1. NFA for $(ab \cup aba)^*$

Mapping NFA's to Regular Expressions

(\Rightarrow We will now show that if a language A is regular, then it is described by a regular expression R such that $L(R) = A$.

Observation: Given an NFA M we can construct an equivalent NFA with:

1. exactly one accept state;
2. no arrows into the start state;
3. no arrows out of the accept state and the accept state is not the same as the start state.

Building a Regular Expression

Given a NFA in the prescribed form, we can create a *generalized non-deterministic FA (GNFA)* $(Q, \Sigma, \delta, q_{start}, q_{accept})$ where

- Edges are labeled by regular expressions (i.e. $\delta : Q \times Q \rightarrow \text{RegExp}(\Sigma)$)
- There are no arrows into q_{start} and no arrows out q_{accept} (and there is only one accept state).
- **Note:** Missing arrows are equivalent to arrows labeled by \emptyset
- A GNFA accepts a string w if we can write $w = w_1 w_2 w_3 \dots w_k$ where $w_i \in \Sigma^*$ and there is a sequence of states $q_0, q_1, q_2, \dots, q_k$ such that $w_i \in L(R_i)$ and $R_i = \delta(q_{i-1}, q_i)$ and $q_0 = q_{start}$ and $q_k = q_{accept}$.

What is the language of a GNFA with only two states?

Example – NFA to Regular Expression

$N = (Q, \Sigma, \delta, q_1, F)$ where

$Q = \{q_1, q_2\}$

$\Sigma = \{a, b\},$

$F = \{q_2\},$ and

δ is specified by the following transition table:

q	a	b
q_1	$\{q_1\}$	$\{q_2\}$
q_2	$\{q_2\}$	$\{q_2\}$

Getting an Equivalent GFNA with Two States

Let $G = (Q, \Sigma, \delta, q_{start}, q_{accept})$ be a GNFA containing at least one state q_t , where $q_t \neq q_{start}, q_{accept}$. We define $G' = (Q', \Sigma, \delta', q_{start}, q_{accept})$ as follows

1. $Q' \leftarrow Q - \{q_t\}$

2. For every $q_i \in Q' - \{q_{accept}\}$, $q_j \in Q' - \{q_{start}\}$, let

$$\delta'(q_i, q_j) = (R_1)(R_2)^*(R_3) \cup (R_4)$$

where $R_1 = \delta(q_i, q_t)$, $R_2 = \delta(q_t, q_t)$, $R_3 = \delta(q_t, q_j)$, and $R_4 = \delta(q_i, q_j)$.

3. **Recall:** $\emptyset^* = \varepsilon$, and for any R , $\varepsilon \cup R = R \cup \varepsilon = R$ and $\emptyset R = R\emptyset = \emptyset$

$$L(G') = L(G)$$

Lemma: The language accepted by G' equals the language accepted by G .

Proof:

- $L(G) \subseteq L(G')$: Every string accepted by G along a path which didn't pass through q_t is unaffected. Otherwise, if we remove q_t from an accepting sequence of states in G , we get an accepting sequence of states in G' : say we have $\dots, q_i, q_t, q_t, \dots, q_t, q_j, \dots$ in G . By the construction, $\delta'(q_i, q_j)$ will include any substring recognized in this subsequence, so \dots, q_i, q_j, \dots will be an accepting computation in G' .
- $L(G') \subseteq L(G)$: if G' accepts a string it must have been accepted by G since a label matching a subsequence of a string accepted by G' corresponds to the concatenation of labels on a path in G .

Removal of all Intermediate States

Theorem: The regular expression on the label of the arrow from q_{start} to q_{start} after all other states have been removed describes the language of the original machine G .

Proof is by induction on the number of states.